@prefix : <http://www.semanticweb.org/socialbenefitapplicant#> .
@prefix ff: <https://foerderfunke.org/default#> .
@prefix owl: <http://www.w3.org/2002/07/owl#> .
@prefix rdf: <http://www.w3.org/1999/02/22-rdf-syntax-ns#> .
@prefix xml: <http://www.w3.org/XML/1998/namespace> .
@prefix xsd: <http://www.w3.org/2001/XMLSchema#> .
@prefix rdfs: <http://www.w3.org/2000/01/rdf-schema#> .
@base <http://www.semanticweb.org/socialbenefitapplicant#> .

<http://www.semanticweb.org/socialbenefitapplicant> rdf:type owl:Ontology .

#################################################################
#    Object Properties
#################################################################

###  https://foerderfunke.org/default#atRiskOfDisabilityType
ff:atRiskOfDisabilityType rdf:type owl:ObjectProperty ;
                          rdfs:domain ff:Person ;
                          rdfs:range ff:Disability ;
                          rdfs:comment "Links a person to a particular type of disability that they risk developing."@en .


###  https://foerderfunke.org/default#cannotSupportThemselvesBecause
ff:cannotSupportThemselvesBecause rdf:type owl:ObjectProperty ;
                                  rdfs:domain ff:Person ;
                                  rdfs:range ff:Disability ;
                                  rdfs:comment "Points to a reason (e.g., Disability) why a person cannot support themselves."@en .


###  https://foerderfunke.org/default#caregiverInHousehold
ff:caregiverInHousehold rdf:type owl:ObjectProperty ;
                        rdfs:domain ff:CareNeed ;
                        rdfs:range ff:Person ;
                        rdfs:comment "Links a care need to a person who can provide the care and lives in the same household as the person who needs care."@en .


###  https://foerderfunke.org/default#causeOfDeath
ff:causeOfDeath rdf:type owl:ObjectProperty ;
                rdfs:domain ff:Person ;
                rdfs:range ff:Event ;
                rdfs:comment "Links a person to an event that  caused their death."@en .


###  https://foerderfunke.org/default#closeRelative
ff:closeRelative rdf:type owl:ObjectProperty ;
                 rdfs:domain ff:Person ;
                 rdfs:range ff:Person ;
                 rdfs:comment "Links a person to another person who is a close relative."@en .


###  https://foerderfunke.org/default#countryOfEmployment
ff:countryOfEmployment rdf:type owl:ObjectProperty ;
                       rdfs:domain ff:Employment ;
                       rdfs:range ff:Country ;
                       rdfs:comment "Defines the country where an employment takes place."@en .


###  https://foerderfunke.org/default#countryOfResidence
ff:countryOfResidence rdf:type owl:ObjectProperty ;
                      rdfs:domain ff:Person ;
                      rdfs:range ff:Country ;
                      rdfs:comment "Links a person to their country of residence."@en .


###  https://foerderfunke.org/default#deceasedCivilPartner
ff:deceasedCivilPartner rdf:type owl:ObjectProperty ;
                        rdfs:domain ff:Person ;
                        rdfs:range ff:Person ;
                        rdfs:comment "Links a person to another person who deceased as their civil partner."@en .


###  https://foerderfunke.org/default#deceasedSpouse
ff:deceasedSpouse rdf:type owl:ObjectProperty ;
                  rdfs:domain ff:Person ;
                  rdfs:range ff:Person ;
                  rdfs:comment "Links a person who deceased as their spouse."@en .


###  https://foerderfunke.org/default#derivesFreedomOfMovementFrom
ff:derivesFreedomOfMovementFrom rdf:type owl:ObjectProperty ;
                                rdfs:domain ff:Person ;
                                rdfs:range ff:Person ;
                                rdfs:comment "Links a person to another person from whom they derive freedom of movement under the Freedom of Movement Act."@en .


###  https://foerderfunke.org/default#employer
ff:employer rdf:type owl:ObjectProperty ;
            rdfs:domain ff:Employment ;
            rdfs:range ff:Employer ;
            rdfs:comment "Links a person to a person or organization that employs them."@en .


###  https://foerderfunke.org/default#fosterChildTo
ff:fosterChildTo rdf:type owl:ObjectProperty ;
                 rdfs:domain ff:Person ;
                 rdfs:range ff:Person ;
                 rdfs:comment "Links a person to their foster parent."@en .


###  https://foerderfunke.org/default#hasChild
ff:hasChild rdf:type owl:ObjectProperty ;
            rdfs:domain ff:Person ;
            rdfs:range ff:Person ;
            rdfs:comment "Links a person to their child."@en .


###  https://foerderfunke.org/default#hasDisabilityType
ff:hasDisabilityType rdf:type owl:ObjectProperty ;
                     rdfs:domain ff:Person ;
                     rdfs:range ff:Disability ;
                     rdfs:comment "Links a person to a particular type of disability that they have."@en .


###  https://foerderfunke.org/default#hasEarningCapacity
ff:hasEarningCapacity rdf:type owl:ObjectProperty ;
                      rdfs:domain ff:Person ;
                      rdfs:range ff:EarningCapacity ;
                      rdfs:comment "Links a person to the status of their earning capacity."@en .


###  https://foerderfunke.org/default#hasEmployment
ff:hasEmployment rdf:type owl:ObjectProperty ;
                 rdfs:domain ff:Person ;
                 rdfs:range ff:Employment ;
                 rdfs:comment "Links a user to a current employment."@en .


###  https://foerderfunke.org/default#hasEmploymentStatus
ff:hasEmploymentStatus rdf:type owl:ObjectProperty ;
                       rdfs:domain ff:Person ;
                       rdfs:range ff:EmploymentStatus ;
                       rdfs:comment "Links a person to their legal employment status."@en .


###  https://foerderfunke.org/default#hasEvent
ff:hasEvent rdf:type owl:ObjectProperty ;
            rdfs:domain ff:Employer ,
                        ff:Person ;
            rdfs:range ff:Event .


###  https://foerderfunke.org/default#hasIncome
ff:hasIncome rdf:type owl:ObjectProperty ;
             rdfs:domain ff:Person ;
             rdfs:range ff:Income ;
             rdfs:comment "Links a person to an object describing their income."@en .


###  https://foerderfunke.org/default#hasInsurance
ff:hasInsurance rdf:type owl:ObjectProperty ;
                rdfs:domain ff:Person ;
                rdfs:range ff:Insurance ;
                rdfs:comment "Links a person to an insurance that they have."@en .


###  https://foerderfunke.org/default#hasMaritalStatus
ff:hasMaritalStatus rdf:type owl:ObjectProperty ;
                    rdfs:domain ff:Person ;
                    rdfs:range ff:MaritalStatus ;
                    rdfs:comment "Links a person to their legal marital status."@en .


###  https://foerderfunke.org/default#hasNoPriorityClaimsOver
ff:hasNoPriorityClaimsOver rdf:type owl:ObjectProperty ;
                           rdfs:domain ff:Person ;
                           rdfs:range ff:SocialBenefit ;
                           rdfs:comment "Links a person to a social benefit if they are not eligible for other benefits with priority over this one."@en .


###  https://foerderfunke.org/default#hasPrimaryCareTaker
ff:hasPrimaryCareTaker rdf:type owl:ObjectProperty ;
                       rdfs:domain ff:Person ;
                       rdfs:range ff:Person ;
                       rdfs:comment "Links a person to a person who has the main responsibility for their living expenses."@en .


###  https://foerderfunke.org/default#hasRehabilitationProvider
ff:hasRehabilitationProvider rdf:type owl:ObjectProperty ;
                             rdfs:domain ff:Person ;
                             rdfs:range ff:RehabilitationProvider ;
                             rdfs:comment "Links a person to their rehabilitation provider."@en .


###  https://foerderfunke.org/default#hasResidencePermit
ff:hasResidencePermit rdf:type owl:ObjectProperty ;
                      rdfs:domain ff:Person ;
                      rdfs:range ff:ResidencePermit ;
                      rdfs:comment "Links a person to a residence permit that they hold."@en .


###  https://foerderfunke.org/default#hasResidenceStatus
ff:hasResidenceStatus rdf:type owl:ObjectProperty ;
                      rdfs:domain ff:Person ;
                      rdfs:range ff:ResidenceStatus ;
                      rdfs:comment "Links a person to their residence status in Germany."@en .


###  https://foerderfunke.org/default#immediateCircleMember
ff:immediateCircleMember rdf:type owl:ObjectProperty ;
                         rdfs:domain ff:Person ;
                         rdfs:range ff:Person ;
                         rdfs:comment "Links a person to another person who is a member of their immediate circle."@en .


###  https://foerderfunke.org/default#incomeTaxCountry
ff:incomeTaxCountry rdf:type owl:ObjectProperty ;
                    rdfs:domain ff:Person ;
                    rdfs:range ff:Country ;
                    rdfs:comment "Links a person to the country where they are subject to income tax."@en .


###  https://foerderfunke.org/default#incomeTaxLiability
ff:incomeTaxLiability rdf:type owl:ObjectProperty ;
                      rdfs:domain ff:Person ;
                      rdfs:range ff:TaxLiabilityScope ;
                      rdfs:comment "Links a person to the scope of their income tax liability."@en .


###  https://foerderfunke.org/default#intendedFundingPeriod
ff:intendedFundingPeriod rdf:type owl:ObjectProperty ;
                         rdfs:domain ff:Training ;
                         rdfs:range ff:Duration ;
                         rdfs:comment "Links something (e.g., a training) to the intended funding period."@en .


###  https://foerderfunke.org/default#isEligibleFor
ff:isEligibleFor rdf:type owl:ObjectProperty ;
                 rdfs:domain ff:Person ;
                 rdfs:range ff:SocialBenefit ;
                 rdfs:comment "Links a person to a service for which they are eligible."@en .


###  https://foerderfunke.org/default#isIneligibleFor
ff:isIneligibleFor rdf:type owl:ObjectProperty ;
                   rdfs:domain ff:Person ;
                   rdfs:range ff:SocialBenefit ;
                   rdfs:comment "Links a person to a service for which they are ineligible."@en .


###  https://foerderfunke.org/default#isNationalOf
ff:isNationalOf rdf:type owl:ObjectProperty ;
                rdfs:domain ff:Person ;
                rdfs:range ff:Country ;
                rdfs:comment "Links a person to a country where they are a national."@en .


###  https://foerderfunke.org/default#legalUnionBeforeEvent
ff:legalUnionBeforeEvent rdf:type owl:ObjectProperty ;
                         rdfs:domain ff:Event ;
                         rdfs:range ff:Person ;
                         rdfs:comment "Links an event (e.g., insurance event), experienced by person A, to another person B with whom they were married or in a civil union before and during the event."@en .


###  https://foerderfunke.org/default#naturalChildTo
ff:naturalChildTo rdf:type owl:ObjectProperty ;
                  rdfs:domain ff:Person ;
                  rdfs:range ff:Person ;
                  rdfs:comment "Links a person to their natural parent."@en .


###  https://foerderfunke.org/default#needsCare
ff:needsCare rdf:type owl:ObjectProperty ;
             rdfs:domain ff:Person ;
             rdfs:range ff:CareNeed ;
             rdfs:comment "Links a person who needs care to a node describing their care needs."@en .


###  https://foerderfunke.org/default#parentalAdress
ff:parentalAdress rdf:type owl:ObjectProperty ;
                  rdfs:domain ff:Person ;
                  rdfs:range ff:Adress ;
                  rdfs:comment "Links a person to the adress of one or more parents."@en .


###  https://foerderfunke.org/default#participates
ff:participates rdf:type owl:ObjectProperty ;
                rdfs:domain ff:Person ;
                rdfs:range ff:Training ;
                rdfs:comment "Links a person to a program, e.g. a formal training, in which they are currently participating."@en .


###  https://foerderfunke.org/default#receivedBenefit
ff:receivedBenefit rdf:type owl:ObjectProperty ;
                   rdfs:domain ff:Person ;
                   rdfs:range ff:SocialBenefit ;
                   rdfs:comment "Links a person to a benefit that they have received in the past."@en .


###  https://foerderfunke.org/default#receivesBenefit
ff:receivesBenefit rdf:type owl:ObjectProperty ;
                   rdfs:domain ff:Person ;
                   rdfs:range ff:SocialBenefit ;
                   rdfs:comment "Links a person to a social benefit that they are currently receiving."@en .


###  https://foerderfunke.org/default#receivesChildBenefitFor
ff:receivesChildBenefitFor rdf:type owl:ObjectProperty ;
                           rdfs:domain ff:Person ;
                           rdfs:range ff:Person ;
                           rdfs:comment "Links a person to a child for which they receive child benefit."@en .


###  https://foerderfunke.org/default#recognizedByLaw
ff:recognizedByLaw rdf:type owl:ObjectProperty ;
                   rdfs:domain ff:Training ;
                   rdfs:range ff:LegalCode ;
                   rdfs:comment "Links something to a law under which it is officially recoginzed."@en .


###  https://foerderfunke.org/default#resultsInTreatment
ff:resultsInTreatment rdf:type owl:ObjectProperty ;
                      rdfs:domain ff:Event ;
                      rdfs:range ff:OccupationalRehabilitation ;
                      rdfs:comment "Describes an event that results in medical treatment."@en .


###  https://foerderfunke.org/default#ruleExemptionBecause
ff:ruleExemptionBecause rdf:type owl:ObjectProperty ;
                        rdfs:domain ff:Training ;
                        rdfs:range ff:Disability ;
                        rdfs:comment "Links something to a reason why it is exempted from a certain rule."@en .


###  https://foerderfunke.org/default#sameHouseholdAs
ff:sameHouseholdAs rdf:type owl:ObjectProperty ;
                   rdfs:domain ff:Person ;
                   rdfs:range ff:Person ;
                   rdfs:comment "Links two persons who live in the same household."@en .


###  https://foerderfunke.org/default#socialSecurityCountry
ff:socialSecurityCountry rdf:type owl:ObjectProperty ;
                         rdfs:domain ff:Person ;
                         rdfs:range ff:Country ;
                         rdfs:comment "Links a person to the country where they are subject to social security."@en .


###  https://foerderfunke.org/default#socialSecurityDuration
ff:socialSecurityDuration rdf:type owl:ObjectProperty ;
                          rdfs:domain ff:Person ;
                          rdfs:range ff:Duration ;
                          rdfs:comment "Links a person to a node describing the duration of their social security obligations."@en .


###  https://foerderfunke.org/default#stepChildTo
ff:stepChildTo rdf:type owl:ObjectProperty ;
               rdfs:domain ff:Person ;
               rdfs:range ff:Person ;
               rdfs:comment "Links a person to their step parent."@en .


###  https://foerderfunke.org/default#subjectToContract
ff:subjectToContract rdf:type owl:ObjectProperty ;
                     rdfs:domain ff:Training ;
                     rdfs:range ff:VocationalTrainingContract ;
                     rdfs:comment "Links something to a type of contract to which it is subject."@en .


###  https://foerderfunke.org/default#triggeringEvent
ff:triggeringEvent rdf:type owl:ObjectProperty ;
                   rdfs:domain ff:EarningCapacity ,
                               ff:OccupationalRehabilitation ;
                   rdfs:range ff:Event ;
                   rdfs:comment "Links something (e.g., earning capacity) to an event that caused it."@en .


###  https://foerderfunke.org/default#wasEligibleFor
ff:wasEligibleFor rdf:type owl:ObjectProperty ;
                  rdfs:domain ff:Person ;
                  rdfs:range ff:SocialBenefit ;
                  rdfs:comment "Links a person to a benefit for which they have been eligible in the past."@en .


###  https://foerderfunke.org/default#wasEntitledToCashBenefitBefore
ff:wasEntitledToCashBenefitBefore rdf:type owl:ObjectProperty ;
                                  rdfs:domain ff:Person ;
                                  rdfs:range ff:Event ;
                                  rdfs:comment "Links a person to an event before which they were entitled to a cash benefit like salary or unemployment benefit."@en .


###  https://foerderfunke.org/default#workforceIntegrationProblemBecause
ff:workforceIntegrationProblemBecause rdf:type owl:ObjectProperty ;
                                      rdfs:domain ff:Person ;
                                      rdfs:range ff:Disability ;
                                      rdfs:comment "Points to a reason (e.g., Disabiltiy) why a person needs support with their integration into the workforce."@en .


#################################################################
#    Data properties
#################################################################

###  https://foerderfunke.org/default#aboveSGBXII41AgeLimit
ff:aboveSGBXII41AgeLimit rdf:type owl:DatatypeProperty ;
                         rdfs:domain ff:Person ;
                         rdfs:range xsd:boolean ;
                         rdfs:comment "True if a person has reached the age limit under § 41 SGB XII, false otherwise."@en .


###  https://foerderfunke.org/default#adequateHealthInsurance
ff:adequateHealthInsurance rdf:type owl:DatatypeProperty ;
                           rdfs:domain ff:Person ;
                           rdfs:range xsd:boolean ;
                           rdfs:comment "True if a person has adequate health insurance cover under the Freedom of Movement Act, false otherwise."@en .


###  https://foerderfunke.org/default#availableForPlacement
ff:availableForPlacement rdf:type owl:DatatypeProperty ;
                         rdfs:domain ff:Person ;
                         rdfs:range xsd:boolean ;
                         rdfs:comment "True if a person is able and willing to work subject to compulsory insurance under normal labor market conditions, false otherwise."@en .


###  https://foerderfunke.org/default#canCoverBasicNeedsOfBenefitUnit
ff:canCoverBasicNeedsOfBenefitUnit rdf:type owl:DatatypeProperty ;
                                   rdfs:domain ff:Person ;
                                   rdfs:range xsd:boolean ;
                                   rdfs:comment "True if a person can cover the basic needs of themselves and the unemployed individuals in their benefit unit with their income, assets, and priority benefits, false otherwise."@en .


###  https://foerderfunke.org/default#canCoverPersonalBasicNeeds
ff:canCoverPersonalBasicNeeds rdf:type owl:DatatypeProperty ;
                              rdfs:domain ff:Person ;
                              rdfs:range xsd:boolean ;
                              rdfs:comment "True if a person can cover their personal basic needs with their income, assets, and priority benefits, false otherwise."@en .


###  https://foerderfunke.org/default#causesLossOfEarnings
ff:causesLossOfEarnings rdf:type owl:DatatypeProperty ;
                        rdfs:domain ff:Event ;
                        rdfs:range xsd:boolean ;
                        rdfs:comment "True if an event causes a loss of earnings for the person experiencing it, false otherwise."@en .


###  https://foerderfunke.org/default#commissionedByEmploymentAgency
ff:commissionedByEmploymentAgency rdf:type owl:DatatypeProperty ;
                                  rdfs:domain ff:Training ;
                                  rdfs:range xsd:boolean ;
                                  rdfs:comment "True if a given training was commissioned by the employment agency, false otherwise."@en .


###  https://foerderfunke.org/default#compulsoryInsuranceFor12In30
ff:compulsoryInsuranceFor12In30 rdf:type owl:DatatypeProperty ;
                                rdfs:domain ff:Person ;
                                rdfs:range xsd:boolean ;
                                rdfs:comment "True if a person has been subject to compulsory insurance for at least 12 months within the last 30 months before registering as unemployed, false otherwise."@en .


###  https://foerderfunke.org/default#eligibleWithinLast3Years
ff:eligibleWithinLast3Years rdf:type owl:DatatypeProperty ;
                            rdfs:domain ff:SocialBenefit ;
                            rdfs:range xsd:boolean ;
                            rdfs:comment "True if a person was eligible for a social benefit within the last 3 years."@en .


###  https://foerderfunke.org/default#employableHoursPerDay
ff:employableHoursPerDay rdf:type owl:DatatypeProperty ;
                         rdfs:domain ff:Person ;
                         rdfs:range xsd:decimal ;
                         rdfs:comment "Links a person to the hours they are able to work per day."@en .


###  https://foerderfunke.org/default#entitledToAsylum
ff:entitledToAsylum rdf:type owl:DatatypeProperty ;
                    rdfs:domain ff:Person ;
                    rdfs:range xsd:boolean ;
                    rdfs:comment "True if a person is entitled to asylum, false otherwise."@en .


###  https://foerderfunke.org/default#entitlesToEmployment
ff:entitlesToEmployment rdf:type owl:DatatypeProperty ;
                        rdfs:domain ff:ResidencePermit ;
                        rdfs:range xsd:boolean ;
                        rdfs:comment "True if a permit entitles to employment, false otherwise."@en .


###  https://foerderfunke.org/default#familyGrossIncome
ff:familyGrossIncome rdf:type owl:DatatypeProperty ;
                     rdfs:domain ff:Income ;
                     rdfs:range xsd:decimal ;
                     rdfs:comment "Points to the amount of family gross income."@en .


###  https://foerderfunke.org/default#fullDayAccompaniment
ff:fullDayAccompaniment rdf:type owl:DatatypeProperty ;
                        rdfs:domain ff:MedicalAccompaniment ;
                        rdfs:range xsd:boolean ;
                        rdfs:comment "A medical accompaniement takes more than 8 hours, including time at the hospital and travel to and from the hospital."@en .


###  https://foerderfunke.org/default#hasAge
ff:hasAge rdf:type owl:DatatypeProperty ;
          rdfs:domain ff:Person ;
          rdfs:range xsd:int ;
          rdfs:comment "Links a person to their age in completed years."@en .


###  https://foerderfunke.org/default#hasAsylumActPermit
ff:hasAsylumActPermit rdf:type owl:DatatypeProperty ;
                      rdfs:domain ff:Person ;
                      rdfs:range xsd:boolean ;
                      rdfs:comment "True if a person has a residence permit under the Asylum Act, false otherwise."@en .


###  https://foerderfunke.org/default#hasConsiderableAssets
ff:hasConsiderableAssets rdf:type owl:DatatypeProperty ;
                         rdfs:domain ff:Person ;
                         rdfs:range xsd:boolean ;
                         rdfs:comment "True if a person has considerable assets under the German Social Code, false otherwise."@en .


###  https://foerderfunke.org/default#hasDate
ff:hasDate rdf:type owl:DatatypeProperty ;
           rdfs:domain ff:Event ;
           rdfs:range xsd:dateTime ;
           rdfs:comment "Links an event to the date when it took place."@en .


###  https://foerderfunke.org/default#hasDisability
ff:hasDisability rdf:type owl:DatatypeProperty ;
                 rdfs:domain ff:Person ;
                 rdfs:range xsd:boolean ;
                 rdfs:comment "True if a person has a disability, false otherwise."@en .


###  https://foerderfunke.org/default#inEmployment
ff:inEmployment rdf:type owl:DatatypeProperty ;
                rdfs:domain ff:Person ;
                rdfs:range xsd:boolean ;
                rdfs:comment "True if a person is currently in an employment relationship, false otherwise."@en .


###  https://foerderfunke.org/default#inPatientCoAdmission
ff:inPatientCoAdmission rdf:type owl:DatatypeProperty ;
                        rdfs:domain ff:MedicalAccompaniment ;
                        rdfs:range xsd:boolean ;
                        rdfs:comment "True if a person is admitted as accompanying person for inpatient treatment, false otherwise."@en .


###  https://foerderfunke.org/default#isFirstVocationalTraining
ff:isFirstVocationalTraining rdf:type owl:DatatypeProperty ;
                             rdfs:domain ff:Training ;
                             rdfs:range xsd:boolean ;
                             rdfs:comment "True if a training instance is a person's first vocational training, false otherwise."@en .


###  https://foerderfunke.org/default#isInTransitionalPeriod
ff:isInTransitionalPeriod rdf:type owl:DatatypeProperty ;
                          rdfs:domain ff:Person ;
                          rdfs:range xsd:boolean ;
                          rdfs:comment "True if a person is in a transitional period of 4 calendar months or less between between two formal educations or after the completion of compulsory military service / community service / voluntary service. False otherwise."@en .


###  https://foerderfunke.org/default#isOpen
ff:isOpen rdf:type owl:DatatypeProperty ;
          rdfs:domain ff:InsolvencyProceeding ;
          rdfs:range xsd:boolean ;
          rdfs:comment "True if a proceeding is open, false otherwise."@en .


###  https://foerderfunke.org/default#isPensionable
ff:isPensionable rdf:type owl:DatatypeProperty ;
                 rdfs:domain ff:Person ;
                 rdfs:range xsd:boolean ;
                 rdfs:comment "True, if a person has reached the legal retirement age, false otherwise."@en .


###  https://foerderfunke.org/default#isPermanent
ff:isPermanent rdf:type owl:DatatypeProperty ;
               rdfs:domain ff:EarningCapacity ;
               rdfs:range xsd:boolean ;
               rdfs:comment "True if a given condition (e.g., earning capacity) is permanent, false otherwise."@en .


###  https://foerderfunke.org/default#isRenumerated
ff:isRenumerated rdf:type owl:DatatypeProperty ;
                 rdfs:domain ff:Event ;
                 rdfs:range xsd:boolean ;
                 rdfs:comment "True if a person is renumerated for an event, false otherwise."@en .


###  https://foerderfunke.org/default#isSingleParent
ff:isSingleParent rdf:type owl:DatatypeProperty ;
                  rdfs:domain ff:Person ;
                  rdfs:range xsd:boolean ;
                  rdfs:comment "True if a person is a single parent, false otherwise."@en .


###  https://foerderfunke.org/default#isVocationalReturnee
ff:isVocationalReturnee rdf:type owl:DatatypeProperty ;
                        rdfs:domain ff:Person ;
                        rdfs:range xsd:boolean ;
                        rdfs:comment "True if a person is a vocational returnee, false otherwise."@en .


###  https://foerderfunke.org/default#lessThanFourMonthsAgo
ff:lessThanFourMonthsAgo rdf:type owl:DatatypeProperty ;
                         rdfs:domain ff:Event ;
                         rdfs:range xsd:boolean ;
                         rdfs:comment "True if an event happened less than four months ago, false otherwise."@en .


###  https://foerderfunke.org/default#monthsAbroad
ff:monthsAbroad rdf:type owl:DatatypeProperty ;
                rdfs:domain ff:Training ;
                rdfs:range xsd:int ;
                rdfs:comment "Links something with a duration (e.g., a training) to the time that it takes place abroad in complete months."@en .


###  https://foerderfunke.org/default#monthsTotal
ff:monthsTotal rdf:type owl:DatatypeProperty ;
               rdfs:domain ff:Duration ;
               rdfs:range xsd:int ;
               rdfs:comment "The total duration of something in completed months."@en .


###  https://foerderfunke.org/default#monthsWithinLast3Years
ff:monthsWithinLast3Years rdf:type owl:DatatypeProperty ;
                          rdfs:domain ff:Duration ;
                          rdfs:range xsd:int ;
                          rdfs:comment "The duration of something within the last three years in compelted months."@en .


###  https://foerderfunke.org/default#newUnionAfterWidowhood
ff:newUnionAfterWidowhood rdf:type owl:DatatypeProperty ;
                          rdfs:domain ff:MaritalStatus ;
                          rdfs:range xsd:boolean ;
                          rdfs:comment "True if a widowed person remarried or entered a new civil union."@en .


###  https://foerderfunke.org/default#obviousLackOfAssets
ff:obviousLackOfAssets rdf:type owl:DatatypeProperty ;
                       rdfs:domain ff:Employer ;
                       rdfs:range xsd:boolean ;
                       rdfs:comment "True if an event coincides with an obvious lack of assets of the thing experiencing the event."@en .


###  https://foerderfunke.org/default#percentAbroad
ff:percentAbroad rdf:type owl:DatatypeProperty ;
                 rdfs:domain ff:Duration ,
                             ff:Training ;
                 rdfs:range xsd:decimal ;
                 rdfs:comment "Links something with a duration (e.g., a training) to the time that it takes place abroad in percentage."@en .


###  https://foerderfunke.org/default#permanentRightOfResidence
ff:permanentRightOfResidence rdf:type owl:DatatypeProperty ;
                             rdfs:domain ff:Person ;
                             rdfs:range xsd:boolean ;
                             rdfs:comment "True if a person has acquired a permanent right of residence under the Freedom of Movement Act, false otherwise."@en .


###  https://foerderfunke.org/default#personalGrossIncome
ff:personalGrossIncome rdf:type owl:DatatypeProperty ;
                       rdfs:domain ff:Income ;
                       rdfs:range xsd:int ;
                       rdfs:comment "Points to the amount of personal gross income."@en .


###  https://foerderfunke.org/default#receivedWithinLast3Years
ff:receivedWithinLast3Years rdf:type owl:DatatypeProperty ;
                            rdfs:domain ff:SocialBenefit ;
                            rdfs:range xsd:boolean ;
                            rdfs:comment "True if a person received a benefit within the last 3 years."@en .


###  https://foerderfunke.org/default#recognizedRefugee
ff:recognizedRefugee rdf:type owl:DatatypeProperty ;
                     rdfs:domain ff:Person ;
                     rdfs:range xsd:boolean ;
                     rdfs:comment "True if a person is a legally recognized refugee, false otherwise."@en .


###  https://foerderfunke.org/default#reducesChildSupplementTo
ff:reducesChildSupplementTo rdf:type owl:DatatypeProperty ;
                            rdfs:domain ff:Income ;
                            rdfs:range xsd:decimal ;
                            rdfs:comment "An applicant's income is offset against child supplement to varying degrees. This property links an income to the amount of child supplement remaining after any income-related reductions are taken into account."@en .


###  https://foerderfunke.org/default#reducesWorkProspectsPermanently
ff:reducesWorkProspectsPermanently rdf:type owl:DatatypeProperty ;
                                   rdfs:domain ff:Disability ;
                                   rdfs:range xsd:boolean ;
                                   rdfs:comment "True if a disability reduces a person's prospect of participating in working life permanently."@en .


###  https://foerderfunke.org/default#reductionDurationInWeeks
ff:reductionDurationInWeeks rdf:type owl:DatatypeProperty ;
                            rdfs:domain ff:EarningCapacity ;
                            rdfs:range xsd:int ;
                            rdfs:comment "Points to the duration in completed weeks for which something (e.g., earning capacity) has been reduced."@en .


###  https://foerderfunke.org/default#reductionInPercent
ff:reductionInPercent rdf:type owl:DatatypeProperty ;
                      rdfs:domain ff:EarningCapacity ;
                      rdfs:range xsd:decimal ;
                      rdfs:comment "Points to the percentage by which something (e.g. earning capacity) is reduced."@en .


###  https://foerderfunke.org/default#rejectedForLackOfAssets
ff:rejectedForLackOfAssets rdf:type owl:DatatypeProperty ;
                           rdfs:domain ff:InsolvencyApplication ;
                           rdfs:range xsd:boolean ;
                           rdfs:comment "True if an insolvency application was rejected for lack of assets, false otherwise."@en .


###  https://foerderfunke.org/default#severeDisability
ff:severeDisability rdf:type owl:DatatypeProperty ;
                    rdfs:domain ff:Disability ;
                    rdfs:range xsd:boolean ;
                    rdfs:comment "True if a disability is severe, false otherwise."@en .


###  https://foerderfunke.org/default#sufficientMeansOfSubsistence
ff:sufficientMeansOfSubsistence rdf:type owl:DatatypeProperty ;
                                rdfs:domain ff:Person ;
                                rdfs:range xsd:boolean ;
                                rdfs:comment "True if a person has sufficient means of subsistence under the Freedom of Movement Act, false otherwise."@en .


###  https://foerderfunke.org/default#tooFarFromTrainingCompany
ff:tooFarFromTrainingCompany rdf:type owl:DatatypeProperty ;
                             rdfs:domain ff:Adress ;
                             rdfs:range xsd:boolean ;
                             rdfs:comment "True if an adress is too far from the user's training company to stay there during training, false otherwise."@en .


###  https://foerderfunke.org/default#unfitForWork
ff:unfitForWork rdf:type owl:DatatypeProperty ;
                rdfs:domain ff:EarningCapacity ;
                rdfs:range xsd:boolean ;
                rdfs:comment "True if a person is unfit for gainful employment, false otherwise."@en ;
                rdfs:label "arbeitsunfähig"@de .


###  https://foerderfunke.org/default#uninterruptedLegalStayForLessThan15Months
ff:uninterruptedLegalStayForLessThan15Months rdf:type owl:DatatypeProperty ;
                                             rdfs:domain ff:Person ;
                                             rdfs:range xsd:boolean ;
                                             rdfs:comment "True if a non-German nationa has been in Germany for less than 15 months without interruption on a permitted, authorized or tolerated basis."@en .


###  https://foerderfunke.org/default#wageCutOffsetMonths
ff:wageCutOffsetMonths rdf:type owl:DatatypeProperty ;
                       rdfs:domain ff:Event ;
                       rdfs:range xsd:int ;
                       rdfs:comment "Links an event to the number of full months within which a wage cut occurred relative to the date of the event. Negative (resp. positive) values indicate a wage cut before (resp. after) the event."@en .


###  https://foerderfunke.org/default#workHoursPerWeek
ff:workHoursPerWeek rdf:type owl:DatatypeProperty ;
                    rdfs:domain ff:Employment ;
                    rdfs:range xsd:decimal ;
                    rdfs:comment "Links a person to the fractional hours they are working on a job per week."@en .


#################################################################
#    Classes
#################################################################

###  https://foerderfunke.org/default#Adress
ff:Adress rdf:type owl:Class .


###  https://foerderfunke.org/default#CareNeed
ff:CareNeed rdf:type owl:Class ;
            rdfs:subClassOf ff:Event .


###  https://foerderfunke.org/default#CommutingAccident
ff:CommutingAccident rdf:type owl:Class ;
                     rdfs:subClassOf ff:Event ;
                     rdfs:comment "An accident on one's way to work."@en ;
                     rdfs:label "Wegeunfall"@de .


###  https://foerderfunke.org/default#Contract
ff:Contract rdf:type owl:Class .


###  https://foerderfunke.org/default#Country
ff:Country rdf:type owl:Class .


###  https://foerderfunke.org/default#Disability
ff:Disability rdf:type owl:Class .


###  https://foerderfunke.org/default#DiscontinuationOfBusiness
ff:DiscontinuationOfBusiness rdf:type owl:Class ;
                             rdfs:subClassOf ff:Event ;
                             rdfs:comment "The complete discontinuation of business activity."@en .


###  https://foerderfunke.org/default#Duration
ff:Duration rdf:type owl:Class .


###  https://foerderfunke.org/default#EEAplusCH
ff:EEAplusCH rdf:type owl:Class ;
             rdfs:subClassOf ff:Country ;
             rdfs:comment "Member states of the European Economic Area (EEA) and Switzerland."@en .


###  https://foerderfunke.org/default#EarningCapacity
ff:EarningCapacity rdf:type owl:Class ;
                   rdfs:comment "Subsumes characteristics of a person's earning capacity."@en ;
                   rdfs:label "Erwerbsfähigkeit"@de .


###  https://foerderfunke.org/default#Employer
ff:Employer rdf:type owl:Class .


###  https://foerderfunke.org/default#Employment
ff:Employment rdf:type owl:Class .


###  https://foerderfunke.org/default#EmploymentStatus
ff:EmploymentStatus rdf:type owl:Class ;
                    rdfs:comment "Instances define a person's legal employment status."@en .


###  https://foerderfunke.org/default#EntryProcedureAndVocationalTrainingArea
ff:EntryProcedureAndVocationalTrainingArea rdf:type owl:Class ;
                                           rdfs:subClassOf ff:Training ;
                                           rdfs:comment "Entry procedure and vocational training in a workshop for people with disabilities or other recognized service providers."@en ;
                                           rdfs:label "Eingangsverfahren und Berufsbildungsbereich"@de .


###  https://foerderfunke.org/default#Event
ff:Event rdf:type owl:Class .


###  https://foerderfunke.org/default#HearingImpairment
ff:HearingImpairment rdf:type owl:Class ;
                     rdfs:subClassOf ff:Disability .


###  https://foerderfunke.org/default#Income
ff:Income rdf:type owl:Class ;
          rdfs:comment "Subsumes characteristics of a person's income situation."@en .


###  https://foerderfunke.org/default#InsolvencyApplication
ff:InsolvencyApplication rdf:type owl:Class ;
                         rdfs:subClassOf ff:Event .


###  https://foerderfunke.org/default#InsolvencyProceeding
ff:InsolvencyProceeding rdf:type owl:Class ;
                        rdfs:subClassOf ff:Event .


###  https://foerderfunke.org/default#Insurance
ff:Insurance rdf:type owl:Class ;
             rdfs:label "Gesetzliche Unfallversicherung"@de .


###  https://foerderfunke.org/default#KindergartenAccident
ff:KindergartenAccident rdf:type owl:Class ;
                        rdfs:subClassOf ff:Event ;
                        rdfs:comment "An accident at kindergarten covered by statutory accident insurance."@en ;
                        rdfs:label "Kindergartenunfall"@de .


###  https://foerderfunke.org/default#LegalCode
ff:LegalCode rdf:type owl:Class .


###  https://foerderfunke.org/default#MaritalStatus
ff:MaritalStatus rdf:type owl:Class ;
                 rdfs:comment "Instances define a person's marital status."@en .


###  https://foerderfunke.org/default#MedicalAccompaniment
ff:MedicalAccompaniment rdf:type owl:Class ;
                        rdfs:subClassOf ff:Event .


###  https://foerderfunke.org/default#MoveToGermany
ff:MoveToGermany rdf:type owl:Class ;
                 rdfs:subClassOf ff:Event .


###  https://foerderfunke.org/default#OccupationalDisease
ff:OccupationalDisease rdf:type owl:Class ;
                       rdfs:subClassOf ff:Event ;
                       rdfs:comment "A recognized occupational disease."@en ;
                       rdfs:label "Berufskrankheit"@de .


###  https://foerderfunke.org/default#OccupationalRehabilitation
ff:OccupationalRehabilitation rdf:type owl:Class ;
                              rdfs:label "Berufliche Rehabilitation"@de .


###  https://foerderfunke.org/default#Person
ff:Person rdf:type owl:Class ;
          rdfs:comment "A human being."@en .


###  https://foerderfunke.org/default#RehabilitationProvider
ff:RehabilitationProvider rdf:type owl:Class ;
                          rdfs:comment "An institution that assumes the costs for a person's rehabilitation."@en ;
                          rdfs:label "zuständiger Rehabilitationsträger"@de .


###  https://foerderfunke.org/default#ResidencePermit
ff:ResidencePermit rdf:type owl:Class ;
                   rdfs:comment "Types of residence permits"@en .


###  https://foerderfunke.org/default#ResidenceStatus
ff:ResidenceStatus rdf:type owl:Class .


###  https://foerderfunke.org/default#School
ff:School rdf:type owl:Class ;
          rdfs:subClassOf ff:Training .


###  https://foerderfunke.org/default#SchoolAccident
ff:SchoolAccident rdf:type owl:Class ;
                  rdfs:subClassOf ff:Event ;
                  rdfs:comment "An accident at school covered by statutory accident insurance."@en ;
                  rdfs:label "Schulunfall"@de .


###  https://foerderfunke.org/default#SocialBenefit
ff:SocialBenefit rdf:type owl:Class ;
                 rdfs:comment "A government program to provide financial support to people under certain conditions."@en .


###  https://foerderfunke.org/default#TaxLiabilityScope
ff:TaxLiabilityScope rdf:type owl:Class ;
                     rdfs:comment "Instances define the scope of a person's tax liability."@en .


###  https://foerderfunke.org/default#Training
ff:Training rdf:type owl:Class ;
            rdfs:comment "Types of formal training or education programs."@en .


###  https://foerderfunke.org/default#VisualImpairment
ff:VisualImpairment rdf:type owl:Class ;
                    rdfs:subClassOf ff:Disability .


###  https://foerderfunke.org/default#VocationalTraining
ff:VocationalTraining rdf:type owl:Class ;
                      rdfs:subClassOf ff:Training ;
                      rdfs:label "Berufsausbildung"@de .


###  https://foerderfunke.org/default#VocationalTrainingContract
ff:VocationalTrainingContract rdf:type owl:Class ;
                              rdfs:subClassOf ff:Contract .


###  https://foerderfunke.org/default#WorkAccident
ff:WorkAccident rdf:type owl:Class ;
                rdfs:subClassOf ff:Event ;
                rdfs:comment "An accident at the work place."@en ;
                rdfs:label "Arbeitsunfall"@de .


#################################################################
#    Individuals
#################################################################

###  https://foerderfunke.org/default#AsylumSeekerBenefits
ff:AsylumSeekerBenefits rdf:type owl:NamedIndividual ,
                                 ff:SocialBenefit .


###  https://foerderfunke.org/default#B100019_LB_102716305
ff:B100019_LB_102716305 rdf:type owl:NamedIndividual ,
                                 ff:SocialBenefit ;
                        rdfs:label "Gesetzliche Unfallversicherung Übergangsgeld"@de ,
                                   "Statutory accident insurance transitional allowance"@en .


###  https://foerderfunke.org/default#B100019_LB_106311931
ff:B100019_LB_106311931 rdf:type owl:NamedIndividual ,
                                 ff:SocialBenefit ;
                        rdfs:label "Bürgergeld"@de ,
                                   "Citizen benefit"@en .


###  https://foerderfunke.org/default#B100019_LB_576842
ff:B100019_LB_576842 rdf:type owl:NamedIndividual ,
                              ff:SocialBenefit ;
                     rdfs:label "Arbeitslosengeld"@de ,
                                "Unemployment benefit"@en .


###  https://foerderfunke.org/default#B100019_LB_576986
ff:B100019_LB_576986 rdf:type owl:NamedIndividual ,
                              ff:SocialBenefit ;
                     rdfs:label "Child allowance"@en ,
                                "Kindergeld"@de .


###  https://foerderfunke.org/default#B100019_LB_581863
ff:B100019_LB_581863 rdf:type owl:NamedIndividual ,
                              ff:SocialBenefit ;
                     rdfs:label "Child supplement"@en ,
                                "Kinderzuschlag"@de .


###  https://foerderfunke.org/default#CivilUnion
ff:CivilUnion rdf:type owl:NamedIndividual ,
                       ff:MaritalStatus .


###  https://foerderfunke.org/default#CraftsCode
ff:CraftsCode rdf:type owl:NamedIndividual ,
                       ff:LegalCode .


###  https://foerderfunke.org/default#Divorced
ff:Divorced rdf:type owl:NamedIndividual .


###  https://foerderfunke.org/default#Employee
ff:Employee rdf:type owl:NamedIndividual ,
                     ff:EmploymentStatus ;
            rdfs:comment "A person who is considered employed by law. May require special clearance (e.g. for relatives of the employer)."@en .


###  https://foerderfunke.org/default#FederalEmploymentAgency
ff:FederalEmploymentAgency rdf:type owl:NamedIndividual ,
                                    ff:RehabilitationProvider ;
                           rdfs:label "Bundesagentur für Arbeit"@de .


###  https://foerderfunke.org/default#FullEarningCapacity
ff:FullEarningCapacity rdf:type owl:NamedIndividual ,
                                ff:EarningCapacity .


###  https://foerderfunke.org/default#Germany
ff:Germany rdf:type owl:NamedIndividual ,
                    ff:Country .


###  https://foerderfunke.org/default#IntegrationAssistance
ff:IntegrationAssistance rdf:type owl:NamedIndividual ,
                                  ff:SocialBenefit .


###  https://foerderfunke.org/default#JobSeeker
ff:JobSeeker rdf:type owl:NamedIndividual ,
                      ff:EmploymentStatus .


###  https://foerderfunke.org/default#L100040_LB_8665924
ff:L100040_LB_8665924 rdf:type owl:NamedIndividual ,
                               ff:SocialBenefit ;
                      rdfs:label "Housing benefit"@en ,
                                 "Wohngeld"@de .


###  https://foerderfunke.org/default#LimitedTaxLiability
ff:LimitedTaxLiability rdf:type owl:NamedIndividual ,
                                ff:TaxLiabilityScope .


###  https://foerderfunke.org/default#MaritimeLabourAct
ff:MaritimeLabourAct rdf:type owl:NamedIndividual ,
                              ff:LegalCode .


###  https://foerderfunke.org/default#Married
ff:Married rdf:type owl:NamedIndividual ,
                    ff:MaritalStatus .


###  https://foerderfunke.org/default#NursingProfessionsAct
ff:NursingProfessionsAct rdf:type owl:NamedIndividual ,
                                  ff:LegalCode .


###  https://foerderfunke.org/default#OpenProceeding
ff:OpenProceeding rdf:type owl:NamedIndividual .


###  https://foerderfunke.org/default#ReducedEarningCapacity
ff:ReducedEarningCapacity rdf:type owl:NamedIndividual ,
                                   ff:EarningCapacity .


###  https://foerderfunke.org/default#RegisteredUnemployed
ff:RegisteredUnemployed rdf:type owl:NamedIndividual ,
                                 ff:EmploymentStatus ;
                        rdfs:comment "A person has officially registered as unemployed with the authorities."@en .


###  https://foerderfunke.org/default#RejectedForLackOfAssets
ff:RejectedForLackOfAssets rdf:type owl:NamedIndividual .


###  https://foerderfunke.org/default#SelfEmployed
ff:SelfEmployed rdf:type owl:NamedIndividual .


###  https://foerderfunke.org/default#SocialAssistance
ff:SocialAssistance rdf:type owl:NamedIndividual ,
                             ff:SocialBenefit .


###  https://foerderfunke.org/default#StatutoryAccidentInsurance
ff:StatutoryAccidentInsurance rdf:type owl:NamedIndividual ,
                                       ff:Insurance .


###  https://foerderfunke.org/default#StatutoryHealthInsurance
ff:StatutoryHealthInsurance rdf:type owl:NamedIndividual ,
                                     ff:Insurance .


###  https://foerderfunke.org/default#Tolerated
ff:Tolerated rdf:type owl:NamedIndividual ,
                      ff:ResidenceStatus ;
             rdfs:label "Geduldet"@de .


###  https://foerderfunke.org/default#TrainingBudget
ff:TrainingBudget rdf:type owl:NamedIndividual ,
                           ff:SocialBenefit .


###  https://foerderfunke.org/default#Unemployed
ff:Unemployed rdf:type owl:NamedIndividual ,
                       ff:EmploymentStatus ;
              rdfs:comment "A person is available for the employment agency's placement efforts and not in employment or in employment for less than 15 hours per week."@en .


###  https://foerderfunke.org/default#UnemploymentBenefitsSVG
ff:UnemploymentBenefitsSVG rdf:type owl:NamedIndividual ,
                                    ff:SocialBenefit ;
                           rdfs:label "Arbeitslosenbeihilfe nach dem Soldatenversorgungsgesetz"@de .


###  https://foerderfunke.org/default#UnfitForWork
ff:UnfitForWork rdf:type owl:NamedIndividual ,
                         ff:EarningCapacity .


###  https://foerderfunke.org/default#UnlimitedTaxLiability
ff:UnlimitedTaxLiability rdf:type owl:NamedIndividual ,
                                  ff:TaxLiabilityScope .


###  https://foerderfunke.org/default#User
ff:User rdf:type owl:NamedIndividual ,
                 ff:Person .


###  https://foerderfunke.org/default#VocationalTrainingAct
ff:VocationalTrainingAct rdf:type owl:NamedIndividual ,
                                  ff:LegalCode .


###  https://foerderfunke.org/default#Widowed
ff:Widowed rdf:type owl:NamedIndividual ,
                    ff:MaritalStatus .


###  Generated by the OWL API (version 4.5.29.2024-05-13T12:11:03Z) https://github.com/owlcs/owlapi
