@prefix : <https://foerderfunke.org/ontologies/socialbenefitontology#> .
@prefix ff: <https://foerderfunke.org/default#> .
@prefix owl: <http://www.w3.org/2002/07/owl#> .
@prefix rdf: <http://www.w3.org/1999/02/22-rdf-syntax-ns#> .
@prefix xml: <http://www.w3.org/XML/1998/namespace> .
@prefix xsd: <http://www.w3.org/2001/XMLSchema#> .
@prefix rdfs: <http://www.w3.org/2000/01/rdf-schema#> .
@base <https://foerderfunke.org/ontologies/socialbenefitontology#> .

<https://foerderfunke.org/ontologies/socialbenefitontology> rdf:type owl:Ontology ;
                                                             owl:versionIRI <https://foerderfunke.org/ontologies/socialbenefitontology/1.0.0> .

#################################################################
#    Object Properties
#################################################################

###  https://foerderfunke.org/default#countryOfEmployment
ff:countryOfEmployment rdf:type owl:ObjectProperty ;
                       rdfs:domain ff:Person ;
                       rdfs:range ff:Country ;
                       rdfs:comment "Links a person to the country where they are employed."@en .


###  https://foerderfunke.org/default#countryOfResidence
ff:countryOfResidence rdf:type owl:ObjectProperty ;
                      rdfs:domain ff:Person ;
                      rdfs:range ff:Country ;
                      rdfs:comment "Links a person to the country where they are a resident."@en .


###  https://foerderfunke.org/default#covers
ff:covers rdf:type owl:ObjectProperty ;
          rdfs:domain ff:Insurance ;
          rdfs:range ff:Event ;
          rdfs:comment "Links an insurance to an event that it covers."@en .


###  https://foerderfunke.org/default#derivesFreedomOfMovementFrom
ff:derivesFreedomOfMovementFrom rdf:type owl:ObjectProperty ;
                                rdfs:domain ff:Person ;
                                rdfs:range ff:Person ;
                                rdfs:comment "Links a non-German national to a relative from whom they derive the right to freedom of movement."@en .


###  https://foerderfunke.org/default#employedBy
ff:employedBy rdf:type owl:ObjectProperty ;
              rdfs:domain ff:Person ;
              rdfs:range ff:Employer ;
              rdfs:comment "Links a person to their employer, which may be another person or an orgnization."@en .


###  https://foerderfunke.org/default#hasChild
ff:hasChild rdf:type owl:ObjectProperty ;
            rdfs:domain ff:Person ;
            rdfs:range ff:Person ;
            rdfs:comment "Links a person to their child."@en .


###  https://foerderfunke.org/default#hasEmploymentStatus
ff:hasEmploymentStatus rdf:type owl:ObjectProperty ;
                       rdfs:domain ff:Person ;
                       rdfs:range ff:EmploymentStatus .


###  https://foerderfunke.org/default#hasEvent
ff:hasEvent rdf:type owl:ObjectProperty ;
            rdfs:comment "Links someone or something to an event that they experienced."@en .


###  https://foerderfunke.org/default#hasIncome
ff:hasIncome rdf:type owl:ObjectProperty ;
             rdfs:domain ff:Person ;
             rdfs:range owl:Thing ;
             rdfs:comment "Links a person to an object describing their income."@en .


###  https://foerderfunke.org/default#hasInsurance
ff:hasInsurance rdf:type owl:ObjectProperty ;
                rdfs:domain ff:Person ;
                rdfs:range ff:Insurance .


###  https://foerderfunke.org/default#hasMaritalStatus
ff:hasMaritalStatus rdf:type owl:ObjectProperty ;
                    rdfs:domain ff:Person ;
                    rdfs:range ff:MaritalStatus ;
                    rdfs:comment "Links a person to an instance describing their marital status."@en .


###  https://foerderfunke.org/default#hasPriorityOver
ff:hasPriorityOver rdf:type owl:ObjectProperty ;
                   rdfs:domain ff:SocialBenefit ;
                   rdfs:range ff:SocialBenefit .


###  https://foerderfunke.org/default#hasRehabilitationProvider
ff:hasRehabilitationProvider rdf:type owl:ObjectProperty ;
                             rdfs:domain ff:Person ;
                             rdfs:range ff:RehabilitationProvider ;
                             rdfs:comment "Links a person to their responsible rehabilitation provider."@en .


###  https://foerderfunke.org/default#hasResidencePermit
ff:hasResidencePermit rdf:type owl:ObjectProperty ;
                      rdfs:domain ff:Person ;
                      rdfs:range ff:ResidencePermit ;
                      rdfs:comment "Links a person to the kind of residence permit that they have."@en .


###  https://foerderfunke.org/default#incomeTaxCountry
ff:incomeTaxCountry rdf:type owl:ObjectProperty ;
                    rdfs:domain ff:Person ;
                    rdfs:range ff:Country ;
                    rdfs:comment "Links a person to the country where they are subject to income tax."@en .


###  https://foerderfunke.org/default#incomeTaxLiability
ff:incomeTaxLiability rdf:type owl:ObjectProperty ;
                      rdfs:domain ff:Person ;
                      rdfs:range ff:TaxLiabilityScope ;
                      rdfs:comment "Links a person to the scope of their income taxliability."@en .


###  https://foerderfunke.org/default#isEligibleFor
ff:isEligibleFor rdf:type owl:ObjectProperty ;
                 rdfs:domain ff:Person ;
                 rdfs:range ff:SocialBenefit .


###  https://foerderfunke.org/default#isNationalOf
ff:isNationalOf rdf:type owl:ObjectProperty ;
                rdfs:domain ff:Person ;
                rdfs:range ff:Country ;
                rdfs:comment "Links a person to a country of their nationality."@en .


###  https://foerderfunke.org/default#ordinaryResidence
ff:ordinaryResidence rdf:type owl:ObjectProperty ;
                     rdfs:domain ff:Person ;
                     rdfs:range ff:Country ;
                     rdfs:comment "Links a person to the country where they ordinarily reside."@en .


###  https://foerderfunke.org/default#participatesIn
ff:participatesIn rdf:type owl:ObjectProperty ;
                  rdfs:domain ff:Person ;
                  rdfs:range ff:Program ;
                  rdfs:comment "Links a person to a program in which they are participating."@en .


###  https://foerderfunke.org/default#plansParticipation
ff:plansParticipation rdf:type owl:ObjectProperty ;
                      rdfs:domain ff:Person ;
                      rdfs:range ff:Program ;
                      rdfs:comment "Links a person to a program in which they plan to participate."@en .


###  https://foerderfunke.org/default#receivesBenefit
ff:receivesBenefit rdf:type owl:ObjectProperty ;
                   rdfs:domain ff:Person ;
                   rdfs:range ff:SocialBenefit ;
                   rdfs:comment "Links a person to a social benefit that they are currently receiving."@en .


###  https://foerderfunke.org/default#reducesEarningCapacity
ff:reducesEarningCapacity rdf:type owl:ObjectProperty ;
                          rdfs:domain ff:Event ;
                          rdfs:range owl:Thing ;
                          rdfs:comment "Links an event to a blanknode describing a reduction in earning capacity that it caused."@en .


###  https://foerderfunke.org/default#sameHouseholdAs
ff:sameHouseholdAs rdf:type owl:ObjectProperty ;
                   rdfs:domain ff:Person ;
                   rdfs:range ff:Person ;
                   rdfs:comment "Links two persons who live in the same household."@en .


###  https://foerderfunke.org/default#socialSecurityCountry
ff:socialSecurityCountry rdf:type owl:ObjectProperty ;
                         rdfs:domain ff:Person ;
                         rdfs:range ff:Country ;
                         rdfs:comment "Links a person to the country where they are subject to social security."@en .


#################################################################
#    Data properties
#################################################################

###  https://foerderfunke.org/default#causedInabilityToWork
ff:causedInabilityToWork rdf:type owl:DatatypeProperty ;
                         rdfs:domain ff:Event ;
                         rdfs:range xsd:boolean ;
                         rdfs:comment "True if an event caused a person to be unable to work. False otherwise."@en .


###  https://foerderfunke.org/default#coversBasicNeeds
ff:coversBasicNeeds rdf:type owl:DatatypeProperty ;
                    rdfs:domain ff:Person ;
                    rdfs:range xsd:boolean ;
                    rdfs:comment "True if a person's income covers the basic needs of themselves and the unemployed individuals in their benefit unit, false otherwise."@en .


###  https://foerderfunke.org/default#durationWeeks
ff:durationWeeks rdf:type owl:DatatypeProperty ;
                 rdfs:domain owl:Thing ;
                 rdfs:range xsd:int ;
                 rdfs:comment "Links something to its duration in weeks, counting each begun week as 1. Example: A value of 3 indicates that the event lasted until some point in its third week."@en .


###  https://foerderfunke.org/default#employableHoursPerDay
ff:employableHoursPerDay rdf:type owl:DatatypeProperty ;
                         rdfs:domain ff:Person ;
                         rdfs:range xsd:decimal ;
                         rdfs:comment "Links a person to the number of hours they are able to work per day."@en .


###  https://foerderfunke.org/default#entitledToAsylum
ff:entitledToAsylum rdf:type owl:DatatypeProperty ;
                    rdfs:domain ff:Person ;
                    rdfs:range xsd:boolean ;
                    rdfs:comment "True if a person is entitled to asylum. False otherwise."@en .


###  https://foerderfunke.org/default#entitlesToEmployment
ff:entitlesToEmployment rdf:type owl:DatatypeProperty ;
                        rdfs:domain owl:Thing ;
                        rdfs:range xsd:boolean ;
                        rdfs:comment "True if a thing (e.g., a residence permit) entitles a person to take up employment in Germany. False otherwise."@en .


###  https://foerderfunke.org/default#familyGrossIncome
ff:familyGrossIncome rdf:type owl:DatatypeProperty ;
                     rdfs:domain owl:Thing ;
                     rdfs:range xsd:decimal ;
                     rdfs:comment "Links a person's income to the amount of family gross income, i.e. all family earnings before deductions and taxes, expressed as a decimal."@en .


###  https://foerderfunke.org/default#hasAge
ff:hasAge rdf:type owl:DatatypeProperty ;
          rdfs:domain ff:Person ;
          rdfs:range xsd:integer ;
          rdfs:comment "A person's age in completed years."@en .


###  https://foerderfunke.org/default#hasDisability
ff:hasDisability rdf:type owl:DatatypeProperty ;
                 rdfs:domain ff:Person ;
                 rdfs:range xsd:boolean ;
                 rdfs:comment "True if a person has a disability, false otherwise"@en .


###  https://foerderfunke.org/default#isPensionable
ff:isPensionable rdf:type owl:DatatypeProperty ;
                 rdfs:domain ff:Person ;
                 rdfs:range xsd:boolean ;
                 rdfs:comment "True if a person has reached the statutory age of retirement, false otherwise."@en .


###  https://foerderfunke.org/default#isSingleParent
ff:isSingleParent rdf:type owl:DatatypeProperty ;
                  rdfs:domain ff:Person ;
                  rdfs:range xsd:boolean ;
                  rdfs:comment "True if the person is a single parent, false otherwise."@en .


###  https://foerderfunke.org/default#moveToGermanyDate
ff:moveToGermanyDate rdf:type owl:DatatypeProperty ;
                     rdfs:domain ff:Person ;
                     rdfs:range xsd:dateTime ;
                     rdfs:comment "Links a person to the date when they moved to Germany."@en .


###  https://foerderfunke.org/default#obviousLackOfAssets
ff:obviousLackOfAssets rdf:type owl:DatatypeProperty ;
                       rdfs:domain owl:Thing ;
                       rdfs:range xsd:boolean ;
                       rdfs:comment "True if someone or something has an obvious lack of assets or experienced an event that coincided with an obvious lack of assets. False otherwise."@en .


###  https://foerderfunke.org/default#permanentRightOfResidence
ff:permanentRightOfResidence rdf:type owl:DatatypeProperty ;
                             rdfs:domain ff:Person ;
                             rdfs:range xsd:boolean ;
                             rdfs:comment "True, if a non-German national has acquired a permanent right of residence in Germany. False otherwise."@en .


###  https://foerderfunke.org/default#personalGrossIncome
ff:personalGrossIncome rdf:type owl:DatatypeProperty ;
                       rdfs:domain owl:Thing ;
                       rdfs:range xsd:decimal ;
                       rdfs:comment "Links a person's income to the amount of personal gross income."@en .


###  https://foerderfunke.org/default#reason
ff:reason rdf:type owl:DatatypeProperty ;
          rdfs:domain owl:Thing ;
          rdfs:range xsd:string ;
          rdfs:comment "Links something to a natural langauge description of its cause."@en .


###  https://foerderfunke.org/default#receivesChildBenefit
ff:receivesChildBenefit rdf:type owl:DatatypeProperty ;
                        rdfs:domain ff:Person ;
                        rdfs:range xsd:decimal ;
                        rdfs:comment "Links a child to the amount of child supplement it receives."@en .


###  https://foerderfunke.org/default#recognizedRefugee
ff:recognizedRefugee rdf:type owl:DatatypeProperty ;
                     rdfs:domain ff:Person ;
                     rdfs:range xsd:boolean ;
                     rdfs:comment "True if a person is a recognized refugee. False otherwise."@en .


###  https://foerderfunke.org/default#reducesChildSupplementTo
ff:reducesChildSupplementTo rdf:type owl:DatatypeProperty ;
                            rdfs:domain owl:Thing ;
                            rdfs:range xsd:decimal ;
                            rdfs:comment "A user's income is offset against child supplement to varying degrees. This property links an income to the amount of child supplement remaining after any income-related reductions are taken into account."@en .


###  https://foerderfunke.org/default#reductionPercentage
ff:reductionPercentage rdf:type owl:DatatypeProperty ;
                       rdfs:domain owl:Thing ;
                       rdfs:range xsd:decimal ;
                       rdfs:comment "Links a reduction to the percentage by which it decreases something."@en .


###  https://foerderfunke.org/default#wageCutOffsetMonths
ff:wageCutOffsetMonths rdf:type owl:DatatypeProperty ;
                       rdfs:domain ff:Event ;
                       rdfs:range xsd:int ;
                       rdfs:comment "Links an event to the number of months within which it caused a wage cut, where negative values indicate a wage cut before and positive values indicate a wage cut after the event. Example: -1 means that a wage cut occurred within the month before the event."@en .


#################################################################
#    Classes
#################################################################

###  https://foerderfunke.org/default#AccidentAtWork
ff:AccidentAtWork rdf:type owl:Class ;
                  rdfs:subClassOf ff:Event ;
                  rdfs:label "Arbeitsunfall"@de .


###  https://foerderfunke.org/default#AccidentOnWayToWork
ff:AccidentOnWayToWork rdf:type owl:Class ;
                       rdfs:subClassOf ff:Event ;
                       rdfs:label "Wegeunfall"@de .


###  https://foerderfunke.org/default#Country
ff:Country rdf:type owl:Class .


###  https://foerderfunke.org/default#DiscontinuationOfBusinessActivity
ff:DiscontinuationOfBusinessActivity rdf:type owl:Class ;
                                     rdfs:subClassOf ff:Event ;
                                     rdfs:comment "A company completely discontinued their business activities."@en .


###  https://foerderfunke.org/default#EEAplusCH
ff:EEAplusCH rdf:type owl:Class ;
             rdfs:subClassOf ff:Country ;
             rdfs:comment "Member states of the European Economic Area (EEA) and Switzerland."@en .


###  https://foerderfunke.org/default#EducationalProgram
ff:EducationalProgram rdf:type owl:Class ;
                      rdfs:subClassOf ff:Program ;
                      rdfs:comment "A program designed for developing certain skills or knowledge."@en .


###  https://foerderfunke.org/default#Employer
ff:Employer rdf:type owl:Class ;
            rdfs:comment "A person or organization that employs one or more persons."@en .


###  https://foerderfunke.org/default#EmploymentStatus
ff:EmploymentStatus rdf:type owl:Class .


###  https://foerderfunke.org/default#Event
ff:Event rdf:type owl:Class ;
         rdfs:comment "A past occurence that marked a change in the circumstances of someone or something."@en .


###  https://foerderfunke.org/default#Insurance
ff:Insurance rdf:type owl:Class .


###  https://foerderfunke.org/default#MaritalStatus
ff:MaritalStatus rdf:type owl:Class ;
                 rdfs:comment "A person's marital status."@en .


###  https://foerderfunke.org/default#OccupationalDisease
ff:OccupationalDisease rdf:type owl:Class ;
                       rdfs:subClassOf ff:Event ;
                       rdfs:label "Berufskrankheit"@de .


###  https://foerderfunke.org/default#OccupationalRehabilitation
ff:OccupationalRehabilitation rdf:type owl:Class ;
                              rdfs:subClassOf ff:Program ;
                              rdfs:comment "A qualified measure for participation in working life."@en .


###  https://foerderfunke.org/default#OpeningInsolvencyProceeding
ff:OpeningInsolvencyProceeding rdf:type owl:Class ;
                               rdfs:subClassOf ff:Event ;
                               rdfs:comment "The competent authority formally opened insolvency proceedgins."@en .


###  https://foerderfunke.org/default#Person
ff:Person rdf:type owl:Class ;
          rdfs:comment "A human being."@en .


###  https://foerderfunke.org/default#Program
ff:Program rdf:type owl:Class ;
           rdfs:comment "Organized measures or activities that a person can participate in."@en .


###  https://foerderfunke.org/default#RehabilitationProvider
ff:RehabilitationProvider rdf:type owl:Class ;
                          rdfs:comment "An institution that assumes the costs for services for social, medical or occupational rehabilitation."@en .


###  https://foerderfunke.org/default#RejectionInsolvencyApplication
ff:RejectionInsolvencyApplication rdf:type owl:Class ;
                                  rdfs:subClassOf ff:Event ;
                                  rdfs:comment "The competent authority rejected a formal request for the initiation of insolvency proceedings."@en .


###  https://foerderfunke.org/default#ResidencePermit
ff:ResidencePermit rdf:type owl:Class .


###  https://foerderfunke.org/default#SocialBenefit
ff:SocialBenefit rdf:type owl:Class ;
                 rdfs:comment "A service, benefit in kind or financial benefit provided for in the German Social Code."@en .


###  https://foerderfunke.org/default#TaxLiabilityScope
ff:TaxLiabilityScope rdf:type owl:Class ;
                     rdfs:comment "Scope of a person's tax liability (limited or unlimited)."@en .


#################################################################
#    Individuals
#################################################################

###  https://foerderfunke.org/default#AnnulledCivilUnion
ff:AnnulledCivilUnion rdf:type owl:NamedIndividual ,
                               ff:MaritalStatus ;
                      rdfs:comment "A person's former civil union has been annulled."@en ;
                      rdfs:label "Annulled civil union"@en .


###  https://foerderfunke.org/default#B100019_LB_106311931
ff:B100019_LB_106311931 rdf:type owl:NamedIndividual ,
                                 ff:SocialBenefit ;
                        rdfs:label "Buergergeld"@de ,
                                   "Citizen benefit"@en .


###  https://foerderfunke.org/default#B100019_LB_574711
ff:B100019_LB_574711 rdf:type owl:NamedIndividual ,
                              ff:SocialBenefit ;
                     rdfs:label "Ausbildungsgeld"@de ,
                                "Training allowance"@en .


###  https://foerderfunke.org/default#B100019_LB_576842
ff:B100019_LB_576842 rdf:type owl:NamedIndividual ,
                              ff:SocialBenefit ;
                     rdfs:label "Arbeitslosengeld"@de ,
                                "Unemployment benefit"@en .


###  https://foerderfunke.org/default#B100019_LB_581863
ff:B100019_LB_581863 rdf:type owl:NamedIndividual ,
                              ff:SocialBenefit ;
                     rdfs:label "Child supplement"@en ,
                                "Kinderzuschlag"@de .


###  https://foerderfunke.org/default#CivilPartnerDeceased
ff:CivilPartnerDeceased rdf:type owl:NamedIndividual ,
                                 ff:MaritalStatus ;
                        rdfs:comment "A person's civil partner is deceased."@en ;
                        rdfs:label "Civil partner deceased"@en .


###  https://foerderfunke.org/default#CivilUnion
ff:CivilUnion rdf:type owl:NamedIndividual ,
                       ff:MaritalStatus ;
              rdfs:comment "A person lives in an active civil union."@en ;
              rdfs:label "Civil union"@en .


###  https://foerderfunke.org/default#Divorced
ff:Divorced rdf:type owl:NamedIndividual ,
                     ff:MaritalStatus ;
            rdfs:comment "A person is divorced."@en .


###  https://foerderfunke.org/default#Employed
ff:Employed rdf:type owl:NamedIndividual ,
                     ff:EmploymentStatus ;
            rdfs:comment "A person with this employment status is legally considered an employee. May require special clearance (e.g., for relatives of the employer)."@en .


###  https://foerderfunke.org/default#FederalEmploymentAgency
ff:FederalEmploymentAgency rdf:type owl:NamedIndividual ,
                                    ff:RehabilitationProvider ;
                           rdfs:label "Bundesagentur für Arbeit"@de ,
                                      "Federal employment agency"@en .


###  https://foerderfunke.org/default#Germany
ff:Germany rdf:type owl:NamedIndividual ,
                    ff:Country ,
                    ff:EEAplusCH .


###  https://foerderfunke.org/default#IndividualInCompanyQualification
ff:IndividualInCompanyQualification rdf:type owl:NamedIndividual ,
                                             ff:EducationalProgram ;
                                    rdfs:label "Individual in-company qualification"@en ,
                                               "Individuelle betriebliche Qualifizierung"@de .


###  https://foerderfunke.org/default#InitialTrainingWDP
ff:InitialTrainingWDP rdf:type owl:NamedIndividual ,
                               ff:EducationalProgram ;
                      rdfs:label "Eingangsverfahren in einer Werkstatt für behinderte Menschen"@de ,
                                 "Initial training in a workshop for disabled people"@en .


###  https://foerderfunke.org/default#JobSeeker
ff:JobSeeker rdf:type owl:NamedIndividual ,
                      ff:EmploymentStatus .


###  https://foerderfunke.org/default#LimitedTaxLiability
ff:LimitedTaxLiability rdf:type owl:NamedIndividual ,
                                ff:TaxLiabilityScope ;
                       rdfs:label "Beschränkt Steuerpflichtig"@de ,
                                  "Limited tax liability"@en .


###  https://foerderfunke.org/default#Married
ff:Married rdf:type owl:NamedIndividual ,
                    ff:MaritalStatus ;
           rdfs:comment "A person is married to another person."@en .


###  https://foerderfunke.org/default#PreVocationalTraining
ff:PreVocationalTraining rdf:type owl:NamedIndividual ,
                                  ff:EducationalProgram ;
                         rdfs:label "Berufsvorbereitende Bildungsmaßnahme"@de ,
                                    "Pre-vocational training"@en .


###  https://foerderfunke.org/default#SelfEmployed
ff:SelfEmployed rdf:type owl:NamedIndividual ,
                         ff:EmploymentStatus .


###  https://foerderfunke.org/default#Single
ff:Single rdf:type owl:NamedIndividual ,
                   ff:MaritalStatus ;
          rdfs:comment "A person is single, i.e. they do not have any other marital status (married, civil union, etc.) recognized by the law."@en .


###  https://foerderfunke.org/default#StatutoryAccidentInsurance
ff:StatutoryAccidentInsurance rdf:type owl:NamedIndividual ,
                                       ff:Insurance .


###  https://foerderfunke.org/default#TransitionalAllowance
ff:TransitionalAllowance rdf:type owl:NamedIndividual ,
                                  ff:SocialBenefit ;
                         rdfs:label "Transitional allowance"@en ,
                                    "Übergangsgeld"@de .


###  https://foerderfunke.org/default#Unemployed
ff:Unemployed rdf:type owl:NamedIndividual ,
                       ff:EmploymentStatus .


###  https://foerderfunke.org/default#UnlimitedTaxLiability
ff:UnlimitedTaxLiability rdf:type owl:NamedIndividual ,
                                  ff:TaxLiabilityScope ;
                         rdfs:label "Unbeschränkte Steuerpflicht"@de ,
                                    "Unlimited tax liability"@en .


###  https://foerderfunke.org/default#User
ff:User rdf:type owl:NamedIndividual ,
                 ff:Person ;
        rdfs:comment "The person who uses the system to check their eligibility for social benefits."@en .


###  https://foerderfunke.org/default#ValidSettlementPermit
ff:ValidSettlementPermit rdf:type owl:NamedIndividual ,
                                  ff:ResidencePermit .


###  https://foerderfunke.org/default#VocationalTraining
ff:VocationalTraining rdf:type owl:NamedIndividual ,
                               ff:EducationalProgram ;
                      rdfs:label "Berufsausbildung"@de ,
                                 "Vocational training"@en .


###  https://foerderfunke.org/default#VocationalTrainingWDP
ff:VocationalTrainingWDP rdf:type owl:NamedIndividual ,
                                  ff:EducationalProgram ;
                         rdfs:label "Berufsbildungsbereich in einer Werkstatt für behinderte Menschen"@de ,
                                    "Vocational training in a workshop for disabled people"@en .


###  https://foerderfunke.org/default#Widowed
ff:Widowed rdf:type owl:NamedIndividual ,
                    ff:MaritalStatus ;
           rdfs:comment "A person's spouse is deceased."@en .


###  Generated by the OWL API (version 4.5.29.2024-05-13T12:11:03Z) https://github.com/owlcs/owlapi
