@prefix ff: <https://foerderfunke.org/default#> .
@prefix owl: <http://www.w3.org/2002/07/owl#> .
@prefix rdf: <http://www.w3.org/1999/02/22-rdf-syntax-ns#> .
@prefix xml: <http://www.w3.org/XML/1998/namespace> .
@prefix xsd: <http://www.w3.org/2001/XMLSchema#> .
@prefix rdfs: <http://www.w3.org/2000/01/rdf-schema#> .
@base <http://www.w3.org/2002/07/owl#> .

[ rdf:type owl:Ontology
 ] .

#################################################################
#    Object Properties
#################################################################

###  https://foerderfunke.org/default#countryOfResidence
ff:countryOfResidence rdf:type owl:ObjectProperty ;
                      rdfs:domain ff:Person ;
                      rdfs:range ff:Country ;
                      rdfs:comment "Links a person to their country of residence."@en .


###  https://foerderfunke.org/default#hasChild
ff:hasChild rdf:type owl:ObjectProperty ;
            rdfs:domain ff:Person ;
            rdfs:range ff:Person ;
            rdfs:comment "Links a person to their child."@en .


###  https://foerderfunke.org/default#hasIncome
ff:hasIncome rdf:type owl:ObjectProperty ;
             rdfs:domain ff:Person ;
             rdfs:range ff:Income ;
             rdfs:comment "Links a person to an object describing their income."@en .


###  https://foerderfunke.org/default#hasMaritalStatus
ff:hasMaritalStatus rdf:type owl:ObjectProperty ;
                    rdfs:domain ff:Person ;
                    rdfs:range ff:MaritalStatus ;
                    rdfs:comment "Links a person to an instance describing their marital status."@en .


###  https://foerderfunke.org/default#hasPriorityOver
ff:hasPriorityOver rdf:type owl:ObjectProperty ;
                   rdfs:domain ff:SocialBenefit ;
                   rdfs:range ff:SocialBenefit .


###  https://foerderfunke.org/default#hasRehabilitationProvider
ff:hasRehabilitationProvider rdf:type owl:ObjectProperty ;
                             rdfs:domain ff:Person ;
                             rdfs:range ff:RehabilitationProvider ;
                             rdfs:comment "Links a person to their responsible rehabilitation provider."@en .


###  https://foerderfunke.org/default#isEligibleFor
ff:isEligibleFor rdf:type owl:ObjectProperty ;
                 rdfs:domain ff:Person ;
                 rdfs:range ff:SocialBenefit .


###  https://foerderfunke.org/default#plansParticipation
ff:plansParticipation rdf:type owl:ObjectProperty ;
                      rdfs:domain ff:Person ;
                      rdfs:range ff:EducationalProgram ;
                      rdfs:comment "Links a person to a program in which they plan to participate."@en .


###  https://foerderfunke.org/default#sameHouseholdAs
ff:sameHouseholdAs rdf:type owl:ObjectProperty ;
                   rdfs:domain ff:Person ;
                   rdfs:range ff:Person ;
                   rdfs:comment "Links two persons who live in the same household."@en .


#################################################################
#    Data properties
#################################################################

###  https://foerderfunke.org/default#coversBasicNeeds
ff:coversBasicNeeds rdf:type owl:DatatypeProperty ;
                    rdfs:domain ff:Income ;
                    rdfs:range xsd:boolean ;
                    rdfs:comment "True if a person's income covers their basic needs, false otherwise."@en .


###  https://foerderfunke.org/default#employableHoursPerDay
ff:employableHoursPerDay rdf:type owl:DatatypeProperty ;
                         rdfs:domain ff:Person ;
                         rdfs:range xsd:float ;
                         rdfs:comment "Links a person to the time they are able to work, in fractional hours per day."@en .


###  https://foerderfunke.org/default#employedHoursPerWeek
ff:employedHoursPerWeek rdf:type owl:DatatypeProperty ;
                        rdfs:domain ff:Person ;
                        rdfs:range xsd:float ;
                        rdfs:comment "Links a person to the time they are in employment, in fractional hours per week."@en .


###  https://foerderfunke.org/default#familyGrossIncome
ff:familyGrossIncome rdf:type owl:DatatypeProperty ;
                     rdfs:domain ff:Income ;
                     rdfs:range xsd:decimal ;
                     rdfs:comment "Links a person's income to the amount of family gross income, i.e. all family earnings before deductions and taxes, expressed as a decimal."@en .


###  https://foerderfunke.org/default#hasAge
ff:hasAge rdf:type owl:DatatypeProperty ;
          rdfs:domain ff:Person ;
          rdfs:range xsd:integer ;
          rdfs:comment "A person's age in completed years."@en .


###  https://foerderfunke.org/default#hasConsiderableAssets
ff:hasConsiderableAssets rdf:type owl:DatatypeProperty ;
                         rdfs:comment "True if a user has considerable assets under the German Code of Social Law, false otherwise."@en .


###  https://foerderfunke.org/default#hasDisability
ff:hasDisability rdf:type owl:DatatypeProperty ;
                 rdfs:domain ff:RehabilitationProvider ;
                 rdfs:range xsd:boolean ;
                 rdfs:comment "True if a person has a disability, false otherwise"@en .


###  https://foerderfunke.org/default#isAbleToWork
ff:isAbleToWork rdf:type owl:DatatypeProperty ;
                rdfs:domain ff:Person ;
                rdfs:range xsd:boolean ;
                rdfs:comment "True if a person is able to take up employment subject to compulsory insurance under normal labor market conditions, false otherwise."@en .


###  https://foerderfunke.org/default#isPensionable
ff:isPensionable rdf:type owl:DatatypeProperty ;
                 rdfs:domain ff:Person ;
                 rdfs:range xsd:boolean ;
                 rdfs:comment "True if a person has reached the statutory age of retirement, false otherwise."@en .


###  https://foerderfunke.org/default#isSingleParent
ff:isSingleParent rdf:type owl:DatatypeProperty ;
                  rdfs:domain ff:Person ;
                  rdfs:range xsd:boolean ;
                  rdfs:comment "True if the person is a single parent, false otherwise."@en .


###  https://foerderfunke.org/default#personalGrossIncome
ff:personalGrossIncome rdf:type owl:DatatypeProperty ;
                       rdfs:domain ff:Income ;
                       rdfs:range xsd:decimal ;
                       rdfs:comment "Links a person's income to the amount of personal gross income, i.e. all personal earnings before deductions and taxes, expressed as a decimal."@en .


###  https://foerderfunke.org/default#receivesChildBenefit
ff:receivesChildBenefit rdf:type owl:DatatypeProperty ;
                        rdfs:range xsd:decimal ;
                        rdfs:comment "Links a child to the amount of child benefit (Kindergeld) it receives."@en .


###  https://foerderfunke.org/default#reducesChildSupplementTo
ff:reducesChildSupplementTo rdf:type owl:DatatypeProperty ;
                            rdfs:domain ff:Income ;
                            rdfs:range xsd:decimal ;
                            rdfs:comment "A user's income is offset against child supplement (Kinderzuschlag) to varying degrees. This property links an income to the amount of child supplement remaining after any income-related reductions are taken into account."@en .


#################################################################
#    Classes
#################################################################

###  https://foerderfunke.org/default#Country
ff:Country rdf:type owl:Class .


###  https://foerderfunke.org/default#EducationalProgram
ff:EducationalProgram rdf:type owl:Class ;
                      rdfs:comment "A program designed for developing certain skills or knowledge."@en .


###  https://foerderfunke.org/default#Income
ff:Income rdf:type owl:Class ;
          rdfs:comment "The general concept of income that may include diverse types of income like assets, gross income, net income, etc."@en .


###  https://foerderfunke.org/default#MaritalStatus
ff:MaritalStatus rdf:type owl:Class ;
                 rdfs:comment "A person's marital status, which may be single, married, widowed, divorced, civil union, annulled civil union, or civil partner deceased."@en .


###  https://foerderfunke.org/default#Person
ff:Person rdf:type owl:Class ;
          rdfs:comment "A human being."@en .


###  https://foerderfunke.org/default#RehabilitationProvider
ff:RehabilitationProvider rdf:type owl:Class ;
                          rdfs:comment "An institution that assumes the costs for services for social, medical or occupational rehabilitation."@en .


###  https://foerderfunke.org/default#SocialBenefit
ff:SocialBenefit rdf:type owl:Class ;
                 rdfs:comment "A service, benefit in kind or financial benefit provided for in the German Social Code."@en .


#################################################################
#    Individuals
#################################################################

###  https://foerderfunke.org/default#AnnulledCivilUnion
ff:AnnulledCivilUnion rdf:type owl:NamedIndividual ,
                               ff:MaritalStatus ;
                      rdfs:comment "A person's former civil union has been annulled."@en ;
                      rdfs:label "Annulled civil union"@en .


###  https://foerderfunke.org/default#B100019_LB_106311931
ff:B100019_LB_106311931 rdf:type owl:NamedIndividual ,
                                 ff:SocialBenefit ;
                        rdfs:label "Buergergeld"@de ,
                                   "Citizen benefit"@en .


###  https://foerderfunke.org/default#B100019_LB_576842
ff:B100019_LB_576842 rdf:type owl:NamedIndividual ,
                              ff:SocialBenefit ;
                     rdfs:label "Arbeitslosengeld"@de ,
                                "Unemployment benefit"@en .


###  https://foerderfunke.org/default#B100019_LB_581863
ff:B100019_LB_581863 rdf:type owl:NamedIndividual ,
                              ff:SocialBenefit ;
                     rdfs:label "Child supplement"@en ,
                                "Kinderzuschlag"@de .


###  https://foerderfunke.org/default#CivilPartnerDeceased
ff:CivilPartnerDeceased rdf:type owl:NamedIndividual ,
                                 ff:MaritalStatus ;
                        rdfs:comment "A person's civil partner is deceased."@en ;
                        rdfs:label "Civil partner deceased"@en .


###  https://foerderfunke.org/default#CivilUnion
ff:CivilUnion rdf:type owl:NamedIndividual ,
                       ff:MaritalStatus ;
              rdfs:comment "A person lives in an active civil union."@en ;
              rdfs:label "Civil union"@en .


###  https://foerderfunke.org/default#Divorced
ff:Divorced rdf:type owl:NamedIndividual ,
                     ff:MaritalStatus ;
            rdfs:comment "A person is divorced."@en .


###  https://foerderfunke.org/default#FederalEmploymentAgency
ff:FederalEmploymentAgency rdf:type owl:NamedIndividual ,
                                    ff:RehabilitationProvider ;
                           rdfs:label "Bundesagentur für Arbeit"@de ,
                                      "Federal employment agency"@en .


###  https://foerderfunke.org/default#Germany
ff:Germany rdf:type owl:NamedIndividual ,
                    ff:Country .


###  https://foerderfunke.org/default#IndividualInCompanyQualification
ff:IndividualInCompanyQualification rdf:type owl:NamedIndividual ,
                                             ff:EducationalProgram ;
                                    rdfs:label "Individual in-company qualification"@en ,
                                               "Individuelle betriebliche Qualifizierung"@de .


###  https://foerderfunke.org/default#InitialTrainingWDP
ff:InitialTrainingWDP rdf:type owl:NamedIndividual ,
                               ff:EducationalProgram ;
                      rdfs:label "Eingangsverfahren in einer Werkstatt für behinderte Menschen"@de ,
                                 "Initial training in a workshop for disabled people"@en .


###  https://foerderfunke.org/default#Married
ff:Married rdf:type owl:NamedIndividual ,
                    ff:MaritalStatus ;
           rdfs:comment "A person is married to another person."@en .


###  https://foerderfunke.org/default#PreVocationalTraining
ff:PreVocationalTraining rdf:type owl:NamedIndividual ,
                                  ff:EducationalProgram ;
                         rdfs:label "Berufsvorbereitende Bildungsmaßnahme"@de ,
                                    "Pre-vocational training"@en .


###  https://foerderfunke.org/default#Single
ff:Single rdf:type owl:NamedIndividual ,
                   ff:MaritalStatus ;
          rdfs:comment "A person is single, i.e. they do not have any other marital status (married, civil union, etc.) recognized by the law."@en .


###  https://foerderfunke.org/default#TransitionalAllowance
ff:TransitionalAllowance rdf:type owl:NamedIndividual ,
                                  ff:SocialBenefit ;
                         rdfs:label "Transitional allowance"@en ,
                                    "Übergangsgeld"@de .


###  https://foerderfunke.org/default#User
ff:User rdf:type owl:NamedIndividual ,
                 ff:Person ;
        rdfs:comment "The person who uses the system to check their eligibility for social benefits."@en .


###  https://foerderfunke.org/default#VocationalTraining
ff:VocationalTraining rdf:type owl:NamedIndividual ,
                               ff:EducationalProgram ;
                      rdfs:label "Berufsausbildung"@de ,
                                 "Vocational training"@en .


###  https://foerderfunke.org/default#VocationalTrainingWDP
ff:VocationalTrainingWDP rdf:type owl:NamedIndividual ,
                                  ff:EducationalProgram ;
                         rdfs:label "Berufsbildungsbereich in einer Werkstatt für behinderte Menschen"@de ,
                                    "Vocational training in a workshop for disabled people"@en .


###  https://foerderfunke.org/default#Widowed
ff:Widowed rdf:type owl:NamedIndividual ,
                    ff:MaritalStatus ;
           rdfs:comment "A person's spouse is deceased."@en .


###  Generated by the OWL API (version 4.5.29.2024-05-13T12:11:03Z) https://github.com/owlcs/owlapi
